qed time fixes

theories/rust_typing/type.v
@@ -63,7 +63,7 @@ Record type `{!typeGS Σ} (rt : Type) := {
   ty_sidecond : iProp Σ;
 
   (* [ty_lfts] is the set of lifetimes that needs to be active for this type to make sense.*)
-  ty_lfts : list lft;
+  _ty_lfts : list lft;
 
   (* [ty_wf_E] is a set of inclusion constraints on lifetimes that need to hold for the type to make sense. *)
   _ty_wf_E : elctx;
@@ -90,7 +90,7 @@ ty_shr_persistent κ π l r : Persistent (ty_shr κ π r l);
     lftE ⊆ E →
     rrust_ctx -∗
     (* We get a token not only for κ, but for all that we might need to recursively use to initiate sharing *)
-    let κ' := lft_intersect_list (ty_lfts) in
+    let κ' := lft_intersect_list (_ty_lfts) in
     q.[κ ⊓ κ'] -∗
     (* [l] needs to be well-layouted *)
     ⌜syn_type_has_layout ty_syn_type ly⌝ -∗
@@ -141,7 +141,6 @@ Arguments ty_own_val {_ _ _}.
 Arguments ty_sidecond {_ _ _}.
 Arguments ty_syn_type {_ _ _}.
 Arguments ty_shr {_ _ _}.
-Arguments ty_lfts {_ _ _} _.
 Arguments ty_share {_ _ _}.
 
 (** We seal [ty_has_op_type] in order to avoid performance issues with automation accidentally unfolding it. *)
@@ -152,13 +151,19 @@ Arguments ty_has_op_type {_ _ _}.
 Lemma ty_op_type_stable `{!typeGS Σ} {rt} (ty : type rt) ot mt :
   ty_has_op_type ty ot mt → syn_type_has_layout ty.(ty_syn_type) (ot_layout ot).
 Proof. rewrite ty_has_op_type_unfold. apply _ty_op_type_stable. Qed.
-Arguments ty_op_type_stable {_ _ _} [_ _ _].
+Global Arguments ty_op_type_stable {_ _ _} [_ _ _].
 
 (** We seal [ty_wf_E] in order to avoid performance issues with Qed time. *)
 Definition ty_wf_E_aux `{!typeGS Σ} : seal (@_ty_wf_E _ _). Proof. by eexists. Qed.
 Definition ty_wf_E `{!typeGS Σ} := ty_wf_E_aux.(unseal).
 Definition ty_wf_E_unfold `{!typeGS Σ} : ty_wf_E = _ty_wf_E := ty_wf_E_aux.(seal_eq).
-Arguments ty_wf_E {_ _ _} _.
+Global Arguments ty_wf_E {_ _ _} _.
+
+(** We seal [ty_lfts] in order to avoid performance issues with Qed time. *)
+Definition ty_lfts_aux `{!typeGS Σ} : seal (@_ty_lfts _ _). Proof. by eexists. Qed.
+Definition ty_lfts `{!typeGS Σ} := ty_lfts_aux.(unseal).
+Definition ty_lfts_unfold `{!typeGS Σ} : ty_lfts = _ty_lfts := ty_lfts_aux.(seal_eq).
+Global Arguments ty_lfts {_ _ _} _.
 
 Lemma ty_memcast_compat `{!typeGS Σ} rt (ty : type rt) ot mt st π r v :
   ty_has_op_type ty ot mt →
@@ -235,14 +240,14 @@ Definition lfts_outlives_E `{!typeGS Σ} (κs : list lft) (κ : lft) : elctx :=
   (λ α, (κ, α)) <$> κs.
 Arguments lfts_outlives_E : simpl never.
 Definition ty_outlives_E `{!typeGS Σ} {rt} (ty : type rt) (κ : lft) : elctx :=
-  lfts_outlives_E ty.(ty_lfts) κ.
+  lfts_outlives_E (ty_lfts ty) κ.
 
 (* TODO this can probably not uphold the invariant that our elctx should be keyed by the LHS of ⊑ₑ *)
 Fixpoint tyl_lfts `{!typeGS Σ} tyl : list lft :=
   match tyl with
   | [] => []
-  | [ty] => ty.(rt_ty).(ty_lfts)
-  | ty :: tyl => ty.(rt_ty).(ty_lfts) ++ tyl.(tyl_lfts)
+  | [ty] => ty_lfts ty.(rt_ty)
+  | ty :: tyl => (ty_lfts ty.(rt_ty)) ++ tyl.(tyl_lfts)
   end.
 
 Fixpoint tyl_wf_E `{!typeGS Σ} tyl : elctx :=
@@ -328,7 +333,7 @@ Program Definition ty_of_st `{!typeGS Σ} rt (st : simple_type rt) : type rt :=
         ▷ st.(st_own) tid r vl ∗
         ⌜syn_type_has_layout st.(st_syn_type) ly⌝ ∗
         ⌜l `has_layout_loc` ly⌝)%I;
-     ty_lfts := [];
+     _ty_lfts := [];
      _ty_wf_E := [];
   |}.
 Next Obligation.
@@ -411,7 +416,7 @@ Section ofe.
       (∀ κ π r l, ty1.(ty_shr) κ π r l ≡ ty2.(ty_shr) κ π r l) →
       (ty1.(ty_syn_type) = ty2.(ty_syn_type)) →
       (ty1.(ty_sidecond) ≡ ty2.(ty_sidecond)) →
-      (ty1.(ty_lfts) = ty2.(ty_lfts)) →
+      (ty_lfts ty1) = (ty_lfts ty2) →
       (ty_wf_E ty1 = ty_wf_E ty2) →
       type_equiv' ty1 ty2.
   Instance type_equiv : Equiv (type rt) := type_equiv'.
@@ -422,7 +427,7 @@ Section ofe.
       (∀ κ π r v, ty1.(ty_shr) κ π r v ≡{n}≡ ty2.(ty_shr) κ π r v) →
       (ty1.(ty_syn_type) = ty2.(ty_syn_type)) →
       (ty1.(ty_sidecond) ≡{n}≡ ty2.(ty_sidecond)) →
-      (ty1.(ty_lfts) = ty2.(ty_lfts)) →
+      (ty_lfts ty1) = (ty_lfts ty2) →
       (ty_wf_E ty1 = ty_wf_E ty2) →
       type_dist' n ty1 ty2.
   Instance type_dist : Dist (type rt) := type_dist'.
@@ -480,7 +485,7 @@ Section ofe.
      ty.(ty_syn_type),
      ty_has_op_type ty,
      ty.(ty_sidecond),
-     ty.(ty_lfts),
+     ty_lfts ty,
      ty_wf_E ty).
   (*
   Program Definition type_pack (x : T) (H : P x) : type rt :=
@@ -730,6 +735,7 @@ Section st_ofe.
       do 7 f_equiv.
       { f_equiv. apply EQ. }
       do 2 f_equiv. apply EQ.
+    - rewrite ty_lfts_unfold. done.
     - rewrite ty_wf_E_unfold. done.
   Qed.
   Global Instance ty_of_st_proper : Proper ((≡) ==> (≡)) (ty_of_st rt).
@@ -752,7 +758,7 @@ Section lft_morph.
     ty_lft_morph_const_α : lft;
     ty_lft_morph_const_E : elctx;
     ty_lft_morph_const_lfts :
-      ⊢ ∀ ty, lft_equiv (lft_intersect_list ((F ty).(ty_lfts))) ty_lft_morph_const_α;
+      ⊢ ∀ ty, lft_equiv (lft_intersect_list (ty_lfts (F ty))) ty_lft_morph_const_α;
     ty_lft_morph_const_wf_E :
       ∀ ty, elctx_interp (ty_wf_E (F ty)) ≡ elctx_interp ty_lft_morph_const_E;
   }.
@@ -767,12 +773,12 @@ Section lft_morph.
     ty_lft_morph_add_E : elctx;
     ty_lft_morph_add_βs : list lft;
     ty_lft_morph_add_lfts :
-      ⊢ ∀ ty, lft_equiv (lft_intersect_list ((F ty).(ty_lfts))) (ty_lft_morph_add_α ⊓ lft_intersect_list ty.(ty_lfts));
+      ⊢ ∀ ty, lft_equiv (lft_intersect_list (ty_lfts (F ty))) (ty_lft_morph_add_α ⊓ lft_intersect_list (ty_lfts ty));
     ty_lft_morph_add_wf_E :
       ∀ ty, elctx_interp (ty_wf_E (F ty)) ≡
           (elctx_interp ty_lft_morph_add_E ∗ elctx_interp (ty_wf_E ty) ∗
             (* some requirements of lifetimes that the type has to outlive *)
-            [∗ list] β ∈ ty_lft_morph_add_βs, β ⊑ lft_intersect_list ty.(ty_lfts))%I;
+            [∗ list] β ∈ ty_lft_morph_add_βs, β ⊑ lft_intersect_list (ty_lfts ty))%I;
   }.
   Existing Class TyLftMorphismAdd.
   Global Arguments mk_lft_morph_add {_ _ _}.
@@ -943,7 +949,7 @@ Section lft_morph.
 
   (* Constructors *)
   Lemma ty_lft_morph_make_id {rt1 rt2} (F : type rt1 → type rt2) :
-    (∀ ty, (F ty).(ty_lfts) = ty.(ty_lfts)) →
+    (∀ ty, ty_lfts (F ty) = ty_lfts ty) →
     (∀ ty, (ty_wf_E (F ty)) = (ty_wf_E ty)) →
     TyLftMorphism F.
   Proof.
@@ -955,7 +961,7 @@ Section lft_morph.
   Qed.
 
   Lemma ty_lft_morph_make_ref {rt1 rt2} (F : type rt1 → type rt2) α :
-    (∀ ty, (F ty).(ty_lfts) = α :: ty.(ty_lfts)) →
+    (∀ ty, ty_lfts (F ty) = α :: (ty_lfts ty)) →
     (∀ ty, (ty_wf_E (F ty)) = (ty_wf_E ty) ++ ty_outlives_E ty α) →
     TyLftMorphism F.
   Proof.
@@ -976,7 +982,7 @@ Section lft_morph.
   Qed.
 
   Lemma ty_lft_morph_make_const {rt1 rt2} (F : type rt1 → type rt2) α E :
-    (∀ ty, (F ty).(ty_lfts) = α) →
+    (∀ ty, ty_lfts (F ty) = α) →
     (∀ ty, (ty_wf_E (F ty)) = E) →
     TyLftMorphism F.
   Proof.
@@ -1909,12 +1915,12 @@ Record DirectLftMorphismAdd {rt1} (Flfts : type rt1 → list lft) (FE : type rt1
   direct_lft_morph_add_E : elctx;
   direct_lft_morph_add_βs : list lft;
   direct_lft_morph_add_lfts :
-    ⊢ ∀ ty, lft_equiv (lft_intersect_list (Flfts ty)) (direct_lft_morph_add_α ⊓ lft_intersect_list ty.(ty_lfts));
+    ⊢ ∀ ty, lft_equiv (lft_intersect_list (Flfts ty)) (direct_lft_morph_add_α ⊓ lft_intersect_list (ty_lfts ty));
   direct_lft_morph_add_wf_E :
     ∀ ty, elctx_interp (FE ty) ≡
         (elctx_interp direct_lft_morph_add_E ∗ elctx_interp (ty_wf_E ty) ∗
           (* some requirements of lifetimes that the type has to outlive *)
-          [∗ list] β ∈ direct_lft_morph_add_βs, β ⊑ lft_intersect_list ty.(ty_lfts))%I;
+          [∗ list] β ∈ direct_lft_morph_add_βs, β ⊑ lft_intersect_list (ty_lfts ty))%I;
 }.
 Global Arguments mk_direct_lft_morph_add {_ _ _}.
 
@@ -1925,7 +1931,7 @@ Inductive DirectLftMorphism {rt1} (Flfts : type rt1 → list lft) (FE : type rt1
 Existing Class DirectLftMorphism.
 
 Global Instance ty_lft_morphism_of_direct {rt1 rt2} (F : type rt1 → type rt2) :
-  DirectLftMorphism (λ ty, (F ty).(ty_lfts)) (λ ty, (ty_wf_E (F ty))) →
+  DirectLftMorphism (λ ty, ty_lfts (F ty)) (λ ty, (ty_wf_E (F ty))) →
   TyLftMorphism F.
 Proof.
   intros [Hm | Hm].
@@ -1938,7 +1944,7 @@ Proof.
 Qed.
 Global Instance ty_lft_morphism_to_direct {rt1 rt2} (F : type rt1 → type rt2) :
   TyLftMorphism F →
-  DirectLftMorphism (λ ty, (F ty).(ty_lfts)) (λ ty, (ty_wf_E (F ty))).
+  DirectLftMorphism (λ ty, ty_lfts (F ty)) (λ ty, (ty_wf_E (F ty))).
 Proof.
   intros [Hm | Hm].
   - apply direct_lft_morph_const.
