theories/rust_typing/automation.v
@@ -1015,7 +1015,7 @@ Ltac solve_goal_normalized_prepare_hook ::=
 
 (** Enum-related tactic calls *)
 Ltac solve_mk_enum_ty_lfts_incl :=
-  unfold_opaque (@ty_lfts); simpl; intros []; set_solver.
+  intros []; rewrite {1}ty_lfts_unfold; simpl; set_solver.
 Ltac solve_mk_enum_ty_wf_E :=
   intros []; rewrite {1}ty_wf_E_unfold/=; set_solver.
 Ltac solve_mk_enum_tag_consistent :=
