theories/rust_typing/enum.v
@@ -113,7 +113,7 @@ Section union.
         ⌜l `has_layout_loc` ul⌝ ∗
         l ◁ₗ{π, κ} r @ ty ∗
         (l +ₗ ly.(ly_size)) ◁ₗ{π, κ} () @ uninit (UntypedSynType $ active_union_rest_ly ul ly))%I;
-    ty_lfts := ty_lfts ty;
+    _ty_lfts := ty_lfts ty;
     _ty_wf_E := ty_wf_E ty;
     ty_sidecond := True;
   |}.
@@ -204,7 +204,7 @@ Section union.
     iDestruct "Htok1" as "(Htok21 & Htok22)".
 
     iPoseProof (ty_share _ E with "[$LFT $TIME $LLCTX] [Htok11 Htok21] [] [] [] Hb1") as "Hb1"; first done.
-    { rewrite -lft_tok_sep. iFrame. }
+    { rewrite ty_lfts_unfold. rewrite -lft_tok_sep. iFrame. }
     { done. }
     { iPureIntro. by eapply has_layout_loc_layout_of_union_member. }
     { iApply (loc_in_bounds_shorten_suf with "Hlb"). done. }
@@ -230,6 +230,7 @@ Section union.
     iIntros "(Hun & Htok1) (Hty & Htok2)".
     simpl. rewrite right_id.
     rewrite -lft_tok_sep.
+    rewrite ty_lfts_unfold.
     iDestruct "Htok2" as "(? & ?)". iFrame.
     iExists ul, ly'. iR. iR. iR. done.
   Qed.
@@ -458,7 +459,7 @@ Section enum.
     _ty_has_op_type ot mt :=
       is_enum_ot e ot mt;
     ty_sidecond := True%I;
-    ty_lfts := e.(enum_lfts);
+    _ty_lfts := e.(enum_lfts);
     _ty_wf_E := e.(enum_wf_E);
   |}.
   Next Obligation.
@@ -512,10 +513,11 @@ Section enum.
     rewrite !lft_tok_sep.
     specialize (syn_type_has_layout_els_sls _ _ Halg) as (sl & Halg'' & ->).
     iPoseProof (ty_share _ E _ _ _ _ _ q'' with "[$] [Htok] [] [] Hlb Hb") as "Hstep"; first done.
-    { simpl. rewrite right_id. done. }
+    { simpl. rewrite !ty_lfts_unfold/=ty_lfts_unfold/=. rewrite right_id. done. }
     { simpl. iPureIntro. by apply use_struct_layout_alg_Some_inv. }
     { done. }
     simpl.
+    rewrite ty_lfts_unfold/=ty_lfts_unfold/=.
     iApply logical_step_fupd.
     iApply (logical_step_wand with "Hstep").
     iModIntro. iIntros "(Hl & Htok)".
@@ -685,8 +687,8 @@ Section ne.
     intros Hen. constructor.
     - simpl. intros. erewrite enum_ne_els; done.
     - apply ty_lft_morphism_of_direct.
-      simpl.
-      rewrite ty_wf_E_unfold.
+      rewrite /=ty_lfts_unfold/=.
+      rewrite /=ty_wf_E_unfold.
       apply enum_ne_lft_mor.
     - rewrite !ty_has_op_type_unfold.
       intros ty ty' Hst Hot ot mt. simpl.
