theories/rust_typing/shr_ref.v
@@ -39,7 +39,7 @@ Section shr_ref.
         inner.(ty_sidecond) ∗
         place_rfn_interp_shared r ri ∗
         &frac{κ'} (λ q, l ↦{q} li) ∗ ▷ □ |={lftE}=> inner.(ty_shr) (κ) π ri li)%I;
-    ty_lfts := [κ] ++ ty_lfts inner;
+    _ty_lfts := [κ] ++ ty_lfts inner;
     _ty_wf_E := ty_wf_E inner ++ ty_outlives_E inner κ;
   |}.
   Next Obligation. iIntros (??????) "(%l & %ly & %r' & -> & ? & ? & ?)". eauto. Qed.
@@ -124,14 +124,13 @@ Section shr_ref.
   Proof.
     constructor; simpl.
     - done.
-    - eapply ty_lft_morph_make_ref; first done.
-      rewrite {1}ty_wf_E_unfold; done.
-    (*- admit.*)
+    - eapply ty_lft_morph_make_ref.
+      + rewrite {1}ty_lfts_unfold; done.
+      + rewrite {1}ty_wf_E_unfold; done.
     - rewrite ty_has_op_type_unfold/=. done.
     - done.
     - solve_type_proper.
     - solve_type_proper.
-  (*Admitted.*)
 Qed.
 
   Global Instance shr_ref_type_ne {rt : Type} κ : TypeNonExpansive (shr_ref (rt:=rt) κ).
