theories/rust_typing/tests.v
@@ -957,7 +957,7 @@ Section test.
     Context (T_ty : type (T_rt)).
 
     Program Definition RawVec_inv_t_inv_spec : ex_inv_def ((RawVec_rt)) ((loc * nat)) := mk_ex_inv_def
-      _ 
+      _
       id
       (λ π inner_rfn '(l, cap) , ⌜inner_rfn = (-[#(l); #(Z.of_nat cap); #(tt)])⌝ ∗ True)%I
       (λ π κ inner_rfn '(l, cap), ⌜inner_rfn = -[#(l); #(Z.of_nat cap); #(tt)]⌝ ∗ True)%I
@@ -996,7 +996,7 @@ Section test.
 
     Program Definition Vec_inv_t_inv_spec : ex_inv_def ((Vec_rt)) (list (place_rfn T_rt)) := mk_ex_inv_def
       (list T_rt)
-      (fmap PlaceIn) 
+      (fmap PlaceIn)
       (λ π inner_rfn 'xs, ∃ (cap : nat) (l : loc), ⌜inner_rfn = -[#((l, cap)); #(Z.of_nat $ length xs)]⌝ ∗ ⌜length xs ≤ cap⌝ ∗ True)%I
       (λ π κ inner_rfn 'xs, ∃ (cap : nat) (l : loc), ⌜inner_rfn = -[#((l, cap)); #(Z.of_nat $ length xs)]⌝ ∗ ⌜length xs ≤ cap⌝ ∗ True)%I
       ([] ++ (ty_lfts T_ty))
